finite character stuff

BourbakiLean2/Set/FiniteCharacter.lean
@@ -42,3 +42,72 @@ instance {s : ι → Set (Set α)} [∀ i, FiniteCharacter $ s i]  : FiniteChara
     constructor
     · exact fun h y hy hf i => h i y hy hf
     · exact fun h i y hy hf => h y hy hf i
+
+instance totally_ordered_finiteCharacter [PartialOrder α] :
+    FiniteCharacter {s : Set α | ∀ x y : s, Comparable x y} where
+  mem_iff_finite_subset_mem {x} := by
+    constructor
+    · intro comp y sub fin ⟨a,h⟩ ⟨b,h'⟩
+      simp only [Comparable, Subtype.le_iff_val]
+      have := comp ⟨a,sub h⟩ ⟨b, sub h'⟩
+      simp only [Comparable, Subtype.le_iff_val] at this
+      exact this
+    · intro fincomp ⟨a,h⟩ ⟨b,h'⟩
+      have : Finite ({a,b} : Set α) := by infer_instance
+      specialize fincomp _ _ this ⟨a,Or.inl rfl⟩ ⟨b, Or.inr rfl⟩
+      · rintro _ (rfl|rfl) <;> assumption
+      · exact fincomp
+
+instance FiniteCharacter.inductiveOrder [FiniteCharacter s] (ne : s.Nonempty) : InductiveOrder s := by
+  apply subset_chain_iUnion_inductive ne
+  intro t ne sub chain
+  rw[mem_iff_finite_subset_mem]
+  intro Y Ysub Yfin
+  by_cases ne' : Y.Nonempty
+  · have this : ∀ y : Y, ∃ z, z ∈ t ∧ y.val ∈ z := by
+      intro ⟨y,memy⟩
+      obtain ⟨⟨i,imem⟩,hi⟩ := Ysub memy
+      exists i
+    obtain ⟨f,hf⟩ := Classical.axiomOfChoice this
+    let Z := f '' Set.univ
+    have : Finite Z := Finite.image _
+    have Zsubt : Z ⊆ t := by
+      intro x hx
+      rw[Set.mem_image_iff] at hx
+      obtain ⟨x,rfl,_⟩ := hx
+      apply (hf x).1
+    obtain ⟨Ymem,hYmem⟩ := ne'
+    have : Nonempty Z := ⟨f ⟨Ymem, hYmem⟩, Set.val_mem_image_of_mem trivial⟩
+    let _inst : TotalOrder Z := by
+      constructor
+      intro ⟨x,memx⟩ ⟨y,memy⟩
+      rw[Set.mem_image_iff] at memx memy
+      obtain ⟨x,rfl,_⟩ := memx
+      obtain ⟨y,rfl,_⟩ := memy
+      have tx := (hf x).1
+      have ty := (hf y).1
+      exact chain _ tx _ ty
+    obtain ⟨g,greatest⟩ := TotalOrder.finite_greatest (α := Z)
+    have bwah (y : Y) : y.val ∈ (g : Set α) := by
+      have : f y ∈ Z := Set.val_mem_image_of_mem trivial
+      have := greatest ⟨_,this⟩
+      simp only [Subtype.le_iff_val, le_set_iff_subset] at this
+      apply this
+      exact (hf _).2
+    have : Y ⊆ (g : Set α) := fun x hx => bwah ⟨x,hx⟩
+    apply (mem_iff_finite_subset_mem (x := g.val)).mp
+    · apply sub
+      apply Zsubt
+      exact g.property
+    · assumption
+    · assumption
+  · obtain ⟨memt, ht⟩ := ne
+    have hs := sub ht
+    rw[Set.nonempty_iff_neq_empty, Ne, Classical.not_not] at ne'
+    rw[ne']
+    rw[mem_iff_finite_subset_mem] at hs
+    specialize hs ∅ Set.empty_subset
+    apply hs inferInstance
+
+theorem FiniteCharacter.has_maximal (h : FiniteCharacter s) (ne : s.Nonempty) : ∃ x : s, Maximal x :=
+  (FiniteCharacter.inductiveOrder ne).has_maximal
